verif/verif_entryindex.v
@@ -53,7 +53,7 @@ Proof.
     + autorewrite with sublist. deadvars!.
       destruct r. autorewrite with norm.
       assert(Z.succ (Zlength c') -1 = Zlength c') by omega. rewrite H1.
-      pose (c'':=map (fun x : node val * index.index => rep_index (snd x)) c'). fold c''.
+      pose (c'':=map (fun x : node val * index.index => Vint(Int.repr(rep_index (snd x)))) c'). fold c''.
       assert (Zlength c'' = Zlength c') by (unfold c''; rewrite Zlength_map; auto).
       rewrite <- H2.
       rewrite Znth_rev_cons by auto.
@@ -61,6 +61,6 @@ Proof.
       unfold cursor_rep.
       Exists (anc_end). Exists (Idx_end). cancel.
       rewrite H2. assert (Zlength ((n, i) :: c') - 1 = Zlength c').
-      rewrite Zlength_cons. omega. rewrite H11.
+      rewrite Zlength_cons. omega. rewrite H10.
       cancel.
 Qed.
