verif/verif_movetonext.v
@@ -28,22 +28,30 @@ Proof.
   forward_if.
   - forward.                    (* t'3=node->numKeys *)
     forward.                    (* return *)
-    Exists ent_end. entailer!.
     destruct isLeaf.
-    + unfold rep_index. reflexivity.
+    + unfold rep_index. entailer!. fold n. rewrite unfold_btnode_rep with (n:=n). unfold n.
+      Exists ent_end. entailer!.
     + simpl in H0. inv H0.
   - forward.                    (* t'2=node->numKeys *)
     forward.                    (* return *)
     { entailer!. unfold node_wf in H.
-      simpl in H. clear -H. admit. (* OK *) }
-    entailer!.
+      simpl in H. clear -H. rewrite Int.signed_repr. rewrite Int.signed_repr.
+      rep_omega. rep_omega. rep_omega. }
     destruct isLeaf.
     + simpl in H0. inv H0.
-    + destruct (numKeys_le le).
-      * unfold rep_index. simpl. Exists ent_end. entailer!.
+    + destruct (numKeys_le le) eqn:HNUM.
+      * unfold rep_index. simpl. entailer!. fold n. rewrite unfold_btnode_rep with (n:=n).
+        unfold n. Exists ent_end. entailer!. simpl. rewrite HNUM. cancel.
       * assert (Z.of_nat (S n0) -1 = Z.of_nat n0).
         { rewrite Nat2Z.inj_succ. rewrite Zsuccminusone. auto. }
-        rewrite H6. unfold rep_index. Exists ent_end. entailer!.
+        rewrite H6. unfold rep_index. entailer!. fold n. rewrite unfold_btnode_rep with (n:=n).
+        unfold n. Exists ent_end. simpl. rewrite HNUM. entailer!.
+Qed.
+
+Lemma complete_sublist_partial: forall (X:Type) (c:cursor X) r i,
+    complete_cursor_correct_rel c r ->
+    partial_cursor_correct_rel (sublist 0 (Zlength c - i) c) r.
+Proof.
 Admitted.
 
 Lemma body_moveToNext: semax_body Vprog Gprog f_moveToNext moveToNext_spec.
@@ -51,39 +59,43 @@ Proof.
   start_function.
   destruct r as [root prel].
   pose (r:=(root,prel)). fold r.
-  destruct c as [|[n i] c'].
-  inv H0. pose (c:=(n,i)::c'). fold c.
+  destruct c as [|[n i] c']. { inv H. inv H2. }
+  pose (c:=(n,i)::c'). fold c.
   unfold cursor_rep. Intros anc_end. Intros idx_end. unfold r.
   forward.                      (* t'17=cursor->relation *)
   unfold relation_rep. Intros.
   forward.                      (* t'18=t'17->numRecords *)
   forward_if.
   {  forward.                   (* return *)
-     assert (numRec = O) by admit. (* OK by H1 *)
      entailer!.
-     unfold moveToNext. simpl. fold c. unfold cursor_rep. Exists anc_end. Exists idx_end. cancel. }
+     unfold moveToNext.
+     assert (get_numrec(root,prel) = O) by admit. rewrite H10.
+     fold c. unfold cursor_rep. Exists anc_end. Exists idx_end. cancel. }
   forward.                      (* skip *)
   forward_call(r,c,pc).         (* t'1=isValid(cursor) *)
   { unfold relation_rep, cursor_rep. unfold r. Exists anc_end. Exists idx_end. cancel.
     change_compspecs CompSpecs. cancel. }
-  forward_if.
+  forward_if.                              (* if t'1 == 0 *)
   { forward.                    (* return *)
-    assert (isValid c r = false) by admit. (* OK by H2 *)
+    destruct (isValid c r) eqn:INVALID. inv H3.
     assert (moveToNext c r = c).
-    { unfold moveToNext. destruct (get_numrec r). auto. rewrite H8. auto. }
+    { unfold moveToNext. destruct (get_numrec r). auto. rewrite INVALID. auto. }
     fold c. fold r. rewrite H9.
     entailer!.  }
   forward.                      (* skip *)
-  assert (isValid c r = true).
-  { destruct (isValid c r). auto. inv H2. } rewrite H3.
+  assert (VALID: isValid c r = true).
+  { destruct (isValid c r). auto. inv H3. } rewrite VALID.
+
   forward_loop
-    (EX i:Z, PROP()
-             LOCAL (temp _t'1 (Val.of_bool true); temp _t'18 (Vint (Int.repr (Z.of_nat numRec))); temp _t'17 prel; temp _cursor pc)
+    (EX i:Z, PROP(up_at_last c = up_at_last (sublist 0 (Zlength c - i) c))
+             LOCAL (temp _t'1 (Val.of_bool true); temp _t'18 (Vint (Int.repr (Z.of_nat (get_numrec (root,prel))))); temp _t'17 prel; temp _cursor pc)
              SEP (relation_rep r; cursor_rep (sublist 0 (Zlength c - i) c) r pc))
     break:(PROP()
-           LOCAL (temp _t'1 (Val.of_bool true); temp _t'18 (Vint (Int.repr (Z.of_nat numRec))); temp _t'17 prel; temp _cursor pc)
+           LOCAL (temp _t'1 (Val.of_bool true); temp _t'18 (Vint (Int.repr (Z.of_nat (get_numrec (root,prel))))); temp _t'17 prel; temp _cursor pc)
            SEP (relation_rep r; cursor_rep (up_at_last c) r pc)).
-  - Exists 0. entailer!. rewrite sublist_same. cancel. auto. omega.
+  - Exists 0. entailer!.
+    + rewrite sublist_same. simpl. auto. auto. omega.
+    + rewrite sublist_same. cancel. auto. omega.
   - Intros i0.
     pose (subc:=sublist 0 (Zlength c - i0) c). fold subc.
     unfold cursor_rep.
@@ -93,44 +105,68 @@ Proof.
     { entailer!. unfold cursor_rep. Exists anc_end0. Exists idx_end0. unfold r. cancel. }
     forward_if (PROP ( )
      LOCAL (temp _t'16 (Vint (Int.repr (Zlength subc - 1))); temp _t'1 (Val.of_bool true);
-            temp _t'18 (Vint (Int.repr (Z.of_nat numRec))); temp _t'17 prel; temp _cursor pc;
-            temp _t'2 (Val.of_bool (andb (Z.gtb (Zlength subc - 1) 0) (index_eqb i (lastpointer n))))) 
-     SEP (cursor_rep subc r pc; relation_rep (root, numRec, depth, prel))).
-    + forward_call(r,subc,pc).     (* t'3=entryInde(cursor) *)
+            temp _t'18 (Vint (Int.repr (Z.of_nat (get_numrec (root,prel))))); temp _t'17 prel; temp _cursor pc;
+            temp _t'2 (Val.of_bool (andb (Z.gtb (Zlength subc - 1) 0) (index_eqb (entryIndex subc) (lastpointer (currNode subc r)))))) 
+     SEP (cursor_rep subc r pc; relation_rep (root, prel))).
+    + assert(PARTIAL: ne_partial_cursor subc r).
+      { unfold complete_cursor in H. destruct H as [CORRECT BALANCED].
+        unfold ne_partial_cursor. split3.
+        - unfold subc. apply complete_sublist_partial. auto.
+        - destruct subc. simpl in H5. inv H5. simpl. omega.
+        - auto. }
+      forward_call(r,subc,pc).     (* t'3=entryIndex(cursor) *)
       { fold r. cancel. }
-      { admit.                  (* todo: cursor_wf preserved *) }
-      forward_call(r,subc,pc).
-      { admit.                  (* todo: cursor_wf preserved *) }
+      forward_call(r,subc,pc).                (* t'4 = curnode(cursor) *)
+      destruct subc as [|[currnode i'] subc'] eqn:HSUBC.
+      { simpl in H5. inv H5. }
+      simpl. assert (SUBNODE: subnode currnode root).
+      { unfold ne_partial_cursor in PARTIAL. destruct PARTIAL.
+        apply partial_cursor_subnode in H6. simpl in H6. auto. }
+      assert(CURRNODE: currnode = currNode subc r). { rewrite HSUBC. simpl. auto. }
       forward_call(currNode subc r). (* 't'5=lastpointer t'4 *)
-      { admit. }
-      { admit.                  (* todo: node_wf preserved *) }
+      { entailer!. }
+      { apply subnode_rep in SUBNODE. rewrite SUBNODE. rewrite CURRNODE. cancel. }
+      { unfold get_root in H1. unfold root_wf in H1. simpl in H1. rewrite <- CURRNODE.
+        apply H1. apply SUBNODE. }
       forward.                  (* t'2= (t'3==t'5) *)
       entailer!.
-      admit.
-      admit.
+      { rewrite Zlength_cons. rewrite Zsuccminusone. 
+        pose (lastp :=  (lastpointer (currNode (sublist 0 (Zlength c - i0) c) r))).
+        fold lastp. rewrite Zlength_cons in H5. rewrite Zsuccminusone in H5.
+        admit.                  (* true from H5 *) }
+      change_compspecs CompSpecs. cancel. apply wand_frame_elim.
     + forward.                  (* t'2=0 *)
       entailer!.
-      admit.
+      rewrite Int.signed_repr in H5.
+      assert(Zlength subc -1 >? 0 = false).
+      { destruct subc. auto. destruct subc. auto. rewrite Zlength_cons in H5.
+        rewrite Zlength_cons in H5. rewrite Zsuccminusone in H5. rewrite Zlength_correct in H5.
+        omega. }
+      rewrite H10. simpl. auto.      
+      admit.                    (* subc length in range *)
     + forward_if.
       * forward.                (* skip *)
         unfold cursor_rep. unfold r. Intros anc_end1. Intros idx_end1.
         forward.                (* t'15=cursor->level *)
         forward.                (* cursor->level = t'15-1 *)
-        { admit. }
+        { entailer!. admit. }   (* length subc in Int range *)
         Exists (i0+1). entailer!. unfold cursor_rep. unfold r.
+        { simpl in H4. rewrite H4. admit. } (* up_at_last conservation *)
         Exists ((getval (currNode subc r))::anc_end1).
-        Exists ((rep_index(entryIndex subc))::idx_end1).
+        Exists ((Vint(Int.repr(rep_index(entryIndex subc))))::idx_end1).
         cancel.
+        rewrite Zlength_sublist. unfold subc. rewrite Zlength_sublist. unfold r.
         admit.                  (* should be ok *)
+        admit. admit. admit. admit.
       * forward.                (* break *)
-        entailer!.
+        entailer!. simpl in H4. rewrite H4. fold subc.
         admit. (* TODO: prove that when the loop stops, we have up_at_last *)
   - unfold cursor_rep. Intros anc_end0. Intros idx_end0. unfold r.
     forward.                    (* t'12=cursor->level *)
     forward.                    (* t'13=cursor->level *)
     forward.                    (* t'14=cursor->ancidx[t'13] *)
-    { admit.                    (* cursor in range *) }
-    { admit. }
+    { entailer!. admit. }       (* up_at_last correct_length *)
+    { entailer!. admit. }
     forward.                    (* cursor->ancestors[t'12] = t'14 +1 *)
     { admit. }
     { admit. }
@@ -140,11 +176,17 @@ Proof.
     Exists anc_end0. Exists idx_end0. cancel. admit. }
     forward_call(r,cincr,pc).       (* t'6=currNode(cursor) *)
     { fold r. cancel. }
-    { admit. }
+    { unfold r. split; auto. admit. }
     destruct (currNode cincr r).
     simpl. Intros.
     (* here I need a representation for the current node of cincr *)
+    (* I will have that once I've proved that cincr is correct cursor *)
     admit.
+Admitted.
+
+Lemma movetonext_complete : forall c r,
+    complete_cursor c r -> complete_cursor (moveToNext c r) r.
+Proof.
 Admitted.
 
 Lemma body_RL_MoveToNext: semax_body Vprog Gprog f_RL_MoveToNext RL_MoveToNext_spec.
@@ -153,38 +195,60 @@ Proof.
   destruct r as [root prel].
   pose (r:=(root,prel)). fold r.
   destruct c as [|[n i] c'].
-  inv H0. pose (c:=(n,i)::c'). fold c.
+  inv H. inv H2. pose (c:=(n,i)::c'). fold c.
   forward_call(r,c,pc).         (* t'1=entryIndex(cursor) *)
   forward_call(r,c,pc).         (* t'2=currNode(cursor) *)
   unfold c. simpl.
   destruct n as [ptr0 le isLeaf First Last pn].
   pose (n:=btnode val ptr0 le isLeaf First Last pn). simpl.
-  assert (subnode n root) by admit. (* I need a cursor correctness property here *)
+  assert (SUBNODE: subnode n root).
+  { unfold complete_cursor in H. destruct H. apply complete_cursor_subnode in H. auto. }
   unfold relation_rep. rewrite subnode_rep with (n:=n) by auto.
-  rewrite unfold_btnode_rep at 1. unfold n. Intros.
+  rewrite unfold_btnode_rep at 1. unfold n. Intros ent_end.
   forward.                      (* t'3=t'2->numKeys *)
   simpl.
   gather_SEP 2 3 4 5. replace_SEP 0 (btnode_rep n).
-  { entailer!. } gather_SEP 0 3. replace_SEP 0 (btnode_rep root).
+  { entailer!. rewrite unfold_btnode_rep with (n:=n). unfold n. Exists ent_end. entailer!. }
+  gather_SEP 0 3. replace_SEP 0 (btnode_rep root).
   { entailer!. apply wand_frame_elim. } gather_SEP 0 1 2. replace_SEP 0 (relation_rep r).
   { entailer!. } fold c.
   forward_if(PROP ( )
      LOCAL (temp _t'3 (Vint (Int.repr (Z.of_nat (numKeys_le le)))); temp _t'2 pn;
-     temp _t'1 (rep_index i); temp _cursor pc)
+     temp _t'1 (Vint(Int.repr(rep_index i))); temp _cursor pc)
      SEP (relation_rep r; match (index_eqb i (ip (numKeys n))) with true => cursor_rep (moveToNext c r) r pc | false => cursor_rep c r pc end)).
   - forward_call(c,pc,r).       (* moveToNext(cursor) *)
     entailer!.
-    assert (i = ip (numKeys_le le)) by admit. (* OK by H2 *)
-    rewrite H10. simpl. admit.                          (* OK *)
+    destruct H. apply complete_correct_rel_index in H.
+    unfold root_wf in H1. apply H1 in SUBNODE. unfold node_wf in SUBNODE. fold n  in H.
+    assert(Z.of_nat (numKeys_le le) <= Z.of_nat Fanout).
+    { simpl in SUBNODE. omega. } simpl in H.
+      destruct i as [|ii].
+    + simpl in H2. simpl in H. clear -H2 H8. apply (f_equal Int.unsigned) in H2.
+      rewrite Fanout_eq in H8. simpl in H8. apply eq_sym in H2. autorewrite with norm in H2.
+      rewrite H2 in H8. exfalso. compute in H8. apply H8. auto.
+    + simpl in H2. apply (f_equal Int.unsigned) in H2. rewrite Fanout_eq in H8. simpl in H8.
+      clear -H2 H8 H. apply eq_sym in H2. simpl in H.
+      autorewrite with norm in H2. apply Nat2Z.inj in H2. subst. simpl.
+      rewrite Nat.eqb_refl. cancel.
   - forward.                                            (* skip *)
-    assert (i <> ip (numKeys n)) by admit. (* OK by H2 *)
-    entailer!. admit.                                   (* OK *)
-  - forward_call(c,pc,r).                               (* moveToNext(cursor) *)
-    + admit.                                            (* false *)
+    destruct H. apply complete_correct_rel_index in H.
+    unfold root_wf in H1. apply H1 in SUBNODE. unfold node_wf in SUBNODE. fold n  in H.
+    assert(Z.of_nat (numKeys_le le) <= Z.of_nat Fanout).
+    { simpl in SUBNODE. omega. } simpl in H.
+    destruct i as [|ii].
+    { entailer!. } unfold index_eqb, numKeys. unfold n.
+    destruct (ii =? numKeys_le le)%nat eqn:HII.
+    + exfalso. apply beq_nat_true in HII. subst. simpl in H2. contradiction.
+    + entailer!.
+  - pose (newc:=if index_eqb i (ip (numKeys n)) then (moveToNext c r) else c).
+    forward_call(newc,pc,r).                               (* moveToNext(cursor) *)
+    + unfold newc. destruct (index_eqb i (ip (numKeys n))); cancel.
+      unfold Frame. simpl. cancel.
+    + split; auto. unfold newc.
+      destruct (index_eqb i (ip (numKeys n))).
+      * apply movetonext_complete. auto.
+      * auto.
     + forward.                                          (* return *)
-      entailer!.
-      * admit.                  (* todo: cursor_wf & cursor_correct preservation *)
-      * admit.                  (* false *)
-Admitted.
-(* Why is there no match in the POSTCONDITION? *)
-        
+      entailer!. unfold newc. simpl.
+      destruct (index_eqb i (ip (numKeys_le le))); fold c; fold r; cancel.
+Qed.
